Proved RHLE sound for arbitrary numbers of programs.

theories/RHLE.v
@@ -6,20 +6,36 @@ Require Import
 Require Import Maps Imp.
 
 Require Import HoareCommon Hoare EHoare.
+Require Import Coq.Vectors.Vector.
 
-Definition Assertion2 := state -> state -> Prop.
+Definition RelAssertion {n m} := Vector.t state n -> Vector.t state m -> Prop.
 
-Definition assert2_implies (P Q : Assertion2) : Prop :=
-  forall st st', P st st' -> Q st st'.
+Definition relAssert_implies {n m} (P Q : RelAssertion) : Prop :=
+  forall (st : Vector.t state n)
+         (st' : Vector.t state m),
+    P st st' -> Q st st'.
 
 Section RHLE.
 
-  Definition rhle_triple (Sigma : ExEnv)
-             (P : Assertion2) (c1 : com) (c2 : com) (Q : Assertion2) : Prop :=
-    forall st1 st2 st1',
-      AllEnv |- st1 =[ c1 ]=> st1'  ->
-                    P st1 st2 ->
-                    exists st2' (exe : AllEnv |- st2 =[ c2 ]=> st2'), Q st1' st2'.
+  Variables n m : nat.
+  Definition Ustate := Vector.t state n.
+  Definition Estate := Vector.t state m.
+
+  Definition Uprogs := Vector.t com n.
+  Definition Eprogs := Vector.t com m.
+
+  Definition rhle_triple
+             (Sigma : ExEnv)
+             (P : RelAssertion)
+             (Uc : Uprogs)
+             (Ec : Eprogs)
+             (Q : RelAssertion) : Prop :=
+    forall (Ust Ust' : Ustate)
+           (Est : Estate),
+      (forall i : Fin.t n,
+          AllEnv |- Vector.nth Ust i =[ Vector.nth Uc i ]=> Vector.nth Ust' i) ->
+      P Ust Est ->
+      exists Est' (exe : forall i, AllEnv |- Vector.nth Est i =[ Vector.nth Ec i ]=> Vector.nth Est' i), Q Ust' Est'.
 
   Notation "Sigma |= {{ P }}  c1 ~# c2  {[ Q ]}" :=
     (rhle_triple Sigma P c1 c2 Q) (at level 90, c1 at next level, c2 at next level)
@@ -28,23 +44,52 @@ Section RHLE.
   Reserved Notation "Sigma , ESigma |- {{ P }}  c1 ~# c2  {[ Q ]}"
            (at level 40, c1 at next level, c2 at next level).
 
-  Inductive rhle_proof Sigma ESigma : Assertion2 -> com -> com -> Assertion2 -> Prop :=
-  | RHE_Skip : forall P,
-      rhle_proof Sigma ESigma P SKIP SKIP P
-  | RHE_SkipIntroL : forall P Q c1 c2,
-      rhle_proof Sigma ESigma P (c1;;SKIP) c2 Q ->
-      rhle_proof Sigma ESigma P c1 c2 Q
-  | RHE_SkipIntroR : forall P Q c1 c2,
-      rhle_proof Sigma ESigma P c1 (c2;;SKIP) Q ->
-      rhle_proof Sigma ESigma P c1 c2 Q
-  | RHE_StepL : forall P Q R c1 c2 c3,
-      (forall st2, hoare_proof Sigma (fun st => P st st2) c1 (fun st => Q st st2)) ->
-      rhle_proof Sigma ESigma Q c2 c3 R ->
-      rhle_proof Sigma ESigma P (c1;;c2) c3 R
-  | RHE_StepR : forall P Q R c1 c2 c3,
-      (forall st1, ehoare_proof ESigma (fun st => P st1 st) c2 (fun st => Q st1 st)) ->
-      rhle_proof Sigma ESigma Q c1 c3 R ->
-      rhle_proof Sigma ESigma P c1 (c2;;c3) R
+  Inductive rhle_proof Sigma ESigma
+    : @RelAssertion n m -> Uprogs -> Eprogs -> @RelAssertion n m -> Prop :=
+  | RHE_Skip : forall P Uc Ec,
+      (forall i, Vector.nth Uc i = CSkip)
+      -> (forall i, Vector.nth Ec i = CSkip)
+      -> rhle_proof Sigma ESigma P Uc Ec P
+
+  | RHE_SkipIntroL : forall P Q Uc Ec Uc' i,
+      (forall i', i <> i' -> Vector.nth Uc i' = Vector.nth Uc' i') ->
+      Vector.nth Uc' i = CSeq (Vector.nth Uc i) CSkip ->
+      rhle_proof Sigma ESigma P Uc' Ec Q ->
+      rhle_proof Sigma ESigma P Uc Ec Q
+
+    | RHE_SkipIntroR : forall P Q Uc Ec Ec' i,
+      (forall i', i <> i' -> Vector.nth Ec i' = Vector.nth Ec' i') ->
+      Vector.nth Ec' i = CSeq (Vector.nth Ec i) CSkip ->
+      rhle_proof Sigma ESigma P Uc Ec' Q ->
+      rhle_proof Sigma ESigma P Uc Ec Q
+
+  | RHE_StepL :
+      forall P Q R Uc Ec Uc' i c1 c2,
+        (forall i', i <> i' -> Vector.nth Uc i' = Vector.nth Uc' i') ->
+        Vector.nth Uc i = CSeq c1 c2 ->
+        Vector.nth Uc' i = c2 ->
+        (forall Ast Est,
+            hoare_proof Sigma (fun st =>
+                                 Vector.nth Ast i = st /\
+                                 P Ast Est) c1
+                        (fun st =>
+                           R (replace Ast i st) Est)) ->
+        rhle_proof Sigma ESigma R Uc' Ec Q ->
+        rhle_proof Sigma ESigma P Uc Ec Q
+
+  | RHE_StepR :
+      forall P Q R Uc Ec Ec' i c1 c2,
+        (forall i', i <> i' -> Vector.nth Ec i' = Vector.nth Ec' i') ->
+        Vector.nth Ec i = CSeq c1 c2 ->
+        Vector.nth Ec' i = c2 ->
+        (forall Ast Est,
+            ehoare_proof ESigma (fun st =>
+                                 Vector.nth Est i = st /\
+                                 P Ast Est) c1
+                        (fun st => R Ast (replace Est i st))) ->
+
+        rhle_proof Sigma ESigma R Uc Ec' Q ->
+        rhle_proof Sigma ESigma P Uc Ec Q
 
   where "Sigma , ESigma |- {{ P }}  c1 ~# c2  {[ Q ]}" := (rhle_proof Sigma ESigma P c1 c2 Q) : hoare_spec_scope.
 
@@ -61,6 +106,30 @@ Section RHLE.
       eapply ehoare_proof_sound in H
     end. *)
 
+  Lemma vector_nth_replace {A} {k}:
+    forall (i : Fin.t k) (v : t A k) (a : A),
+      nth (replace v i a) i = a.
+  Proof.
+    induction i;
+      intros; pattern v; eapply caseS'; eauto; intros.
+    simpl; eauto.
+  Qed.
+
+  Lemma vector_nth_replace' {A} {k}:
+    forall (i i0 : Fin.t k) (v : t A k) (a : A),
+      i <> i0 ->
+      nth (replace v i a) i0 = nth v i0.
+  Proof.
+    induction i0;
+      intros; pattern v; eapply caseS'; eauto; intros.
+    - simpl; revert v a H h t.
+      pattern i; eapply Fin.caseS'; intros; eauto.
+      congruence.
+    - simpl; revert v a H h t.
+      pattern i; eapply Fin.caseS'; intros; eauto.
+      eapply IHi0; congruence.
+  Qed.
+
   Theorem rhle_proof_sound Sigs Sigma ESigma
           (Cons_Env : Consistent_Env {| AllEnv := {| funSigs := Sigs; funSpecs := Sigma; funDefs := empty |}; funExSpecs := ESigma |})
     : forall P c1 c2 Q,
@@ -70,22 +139,72 @@ Section RHLE.
   Proof.
     intros ? ? ? ? pf.
     unfold rhle_triple.
-    induction pf; intros st1 st2 st1' exe HP.
-    - inversion exe; subst; eauto.
-    - firstorder eauto.
-    - edestruct IHpf as [st2' [exe' HQ]]; eauto.
-      inversion exe'; subst; eauto.
-      inversion X0; subst.
-      eexists _, X; eauto.
-    - inversion exe; subst; edestruct IHpf; eauto.
-      eapply hoare_proof_sound in H; eauto.
-    - eapply (@ehoare_proof_link {| AllEnv := {| funSigs := Sigs; funSpecs := Sigma; funDefs := empty |}; funExSpecs := ESigma |}) in H; eauto using productive_empty.
-      edestruct H as [st' [exe' HQ]]; eauto.
-      edestruct IHpf as [st2' [? ?]]; eauto.
+    induction pf; intros Ust Ust' Est exe HP.
+    - eexists Est.
+      assert (Ust' = Ust).
+      { revert H exe; clear.
+        unfold Ustate in *; revert Ust Ust'.
+        induction Uc.
+        - intro; pattern Ust; eapply VectorDef.case0.
+          intro; pattern Ust'; eapply VectorDef.case0.
+          eauto.
+        - intro; pattern Ust; eapply VectorDef.caseS'.
+          intros h0 t Ust'; pattern Ust'; eapply VectorDef.caseS'.
+          intros; f_equal.
+          + specialize (H Fin.F1); specialize (exe Fin.F1); simpl in *.
+            subst; inversion exe; eauto.
+          + eapply IHUc; intros; eauto.
+            eapply (fun i => H (Fin.FS i)).
+            eapply (fun i => exe (Fin.FS i)).
+      }
+      assert (forall (i : Fin.t m), ceval {| funSigs := Sigs; funSpecs := Sigma; funDefs := @empty funDef |}  (nth Ec i) (nth Est i) (nth Est i)).
+      { revert H0; clear.
+        intros.
+        rewrite H0.
+        econstructor.
+      }
+      eexists X; subst; eauto.
+    - eapply IHpf; eauto.
+      intros.
+      destruct (Fin.eq_dec i i0); subst.
+      + rewrite H0; eauto.
+      + rewrite <- H by eauto.
+        eapply exe.
+    - edestruct IHpf as [Est' [exe' HQ]]; eauto.
+      assert (forall (i0 : Fin.t m), ceval {| funSigs := Sigs; funSpecs := Sigma; funDefs := @empty funDef |} (nth Ec i0) (nth Est i0)  (nth Est' i0) ).
+      { intros; destruct (Fin.eq_dec i i0); subst.
+        + specialize (exe' i0); rewrite H0 in exe'; simpl in *.
+          inversion exe'; subst.
+          inversion X0; subst.
+          eauto.
+        + rewrite H by eauto.
+          eapply exe'.
+      }
+      eauto.
+    - generalize (exe i); intros exe'.
+      rewrite H0 in exe'; inversion exe'; subst.
+      edestruct (IHpf (replace Ust i st') Ust'); eauto.
+      + intros; destruct (Fin.eq_dec i i0); subst.
+        * rewrite vector_nth_replace; eauto.
+        * rewrite vector_nth_replace', <- H; eauto.
+      + eapply (hoare_proof_sound _ _ _ _ _ (H2 Ust Est) _ _ X); eauto.
+    - specialize (H2 Ust Est).
+      eapply (@ehoare_proof_link {| AllEnv := {| funSigs := Sigs; funSpecs := Sigma; funDefs := empty |}; funExSpecs := ESigma |}) in H2; eauto using productive_empty.
+      edestruct H2 as [? [? ?] ]; try tauto.
+      edestruct IHpf as [Est' [exe' HQ]]; eauto.
+      assert (forall (i0 : Fin.t m), ceval {| funSigs := Sigs; funSpecs := Sigma; funDefs := @empty funDef |}
+                                           (nth Ec i0)
+                                           (nth Est i0)
+                                           (nth Est' i0)); eauto.
+      intros; destruct (Fin.eq_dec i i0); subst.
+      + rewrite H0; econstructor; eauto.
+        specialize (exe' i0); rewrite vector_nth_replace in exe'; eauto.
+      + specialize (exe' i0); rewrite vector_nth_replace' in exe'; eauto.
+        rewrite H; eauto.
   Qed.
 
-  Definition rwp (Sigma : Env) c (Q : Assertion2) : Assertion2 :=
-    fun st1 st2 => exists st2' (exe : Sigma |- st2 =[ c ]=> st2'), Q st1 st2'.
+  (* Definition rwp (Sigma : Env) c (Q : Assertion2) : Assertion2 :=
+    fun st1 st2 => exists st2' (exe : Sigma |- st2 =[ c ]=> st2'), Q st1 st2'. *)
 
         (* Need to adjust this proof to align with new semantics. *)
   (*Theorem rhle_proof_complete Sigs Sigma : forall P c1 c2 Q,
@@ -104,6 +223,15 @@ Section RHLE.
   Admitted. *)
 
 End RHLE.
+
+(*Lemma existential_not_universal :
+    ~(forall Sigma P Q p, (~ (hoare_triple Sigma P p (fun st => ~ Q st)) ->
+        (ehoare_triple Sigma P p Q))).
+Proof.
+  unfold not; intros.
+  assert  *)
+
+
 
 Notation "Sigma |= {{ P }}  c1 ~# c2  {[ Q ]}" :=
   (rhle_triple Sigma P c1 c2 Q) (at level 90, c1 at next level, c2 at next level)
